CollapsingTowers/TwoLevel/Typing.lean
@@ -7,33 +7,57 @@ def binds (x : ℕ) (τ : Ty) (Γ : TEnv) :=
   indexr x Γ = some τ
 
 inductive typing : TEnv -> Expr -> Ty -> Prop where
-  | fvar : ∀ Γ x τ, binds x τ Γ -> typing Γ (.fvar x) τ
-  | lam₁ : ∀ Γ e τ𝕒 τ𝕓, typing (τ𝕒 :: Γ) (open₀ Γ.length e) τ𝕓 -> Γ.length ∉ fv e -> typing Γ (.lam₁ e) (.arrow τ𝕒 τ𝕓)
-  |
-  lam₂ :
-    ∀ Γ e τ𝕒 τ𝕓,
-      typing (.rep τ𝕒 :: Γ) (open₀ Γ.length e) (.rep τ𝕓) -> Γ.length ∉ fv e -> typing Γ (.lam₂ e) (.rep (.arrow τ𝕒 τ𝕓))
-  | app₁ : ∀ Γ f arg τ𝕒 τ𝕓, typing Γ f (.arrow τ𝕒 τ𝕓) -> typing Γ arg τ𝕒 -> typing Γ (.app₁ f arg) τ𝕓
-  |
-  app₂ : ∀ Γ f arg τ𝕒 τ𝕓, typing Γ f (.rep (.arrow τ𝕒 τ𝕓)) -> typing Γ arg (.rep τ𝕒) -> typing Γ (.app₂ f arg) (.rep τ𝕓)
-  | plus₁ : ∀ Γ l r, typing Γ l .nat -> typing Γ r .nat -> typing Γ (.plus₁ l r) .nat
-  | plus₂ : ∀ Γ l r, typing Γ l (.rep .nat) -> typing Γ r (.rep .nat) -> typing Γ (.plus₂ l r) (.rep .nat)
-  | lit₁ : ∀ Γ n, typing Γ (.lit₁ n) .nat
-  | lit₂ : ∀ Γ n, typing Γ (.lit₂ n) (.rep .nat)
-  | code : ∀ Γ e τ, typing Γ e τ -> typing Γ (.code e) (.rep τ)
-  | reflect : ∀ Γ e τ, typing Γ e τ -> typing Γ (.reflect e) (.rep τ)
-  |
-  lam𝕔 :
-    ∀ Γ e τ𝕒 τ𝕓,
-      typing (τ𝕒 :: Γ) (open₀ Γ.length e) (.rep τ𝕓) -> Γ.length ∉ fv e -> typing Γ (.lam𝕔 e) (.rep (.arrow τ𝕒 τ𝕓))
-  |
-  lets :
-    ∀ Γ b e τ𝕒 τ𝕓, typing Γ b τ𝕒 -> typing (τ𝕒 :: Γ) (open₀ Γ.length e) τ𝕓 -> Γ.length ∉ fv e -> typing Γ (.lets b e) τ𝕓
-  |
-  let𝕔 :
-    ∀ Γ b e τ𝕒 τ𝕓,
-      typing Γ b τ𝕒 ->
-        typing (τ𝕒 :: Γ) (open₀ Γ.length e) (.rep τ𝕓) -> Γ.length ∉ fv e -> typing Γ (.let𝕔 b e) (.rep τ𝕓)
+  | fvar : ∀ Γ x τ,
+    binds x τ Γ ->
+    typing Γ (.fvar x) τ
+  | lam₁ : ∀ Γ e τ𝕒 τ𝕓,
+    typing (τ𝕒 :: Γ) (open₀ Γ.length e) τ𝕓 ->
+    Γ.length ∉ fv e ->
+    typing Γ (.lam₁ e) (.arrow τ𝕒 τ𝕓)
+  | lam₂ : ∀ Γ e τ𝕒 τ𝕓,
+    typing (.rep τ𝕒 :: Γ) (open₀ Γ.length e) (.rep τ𝕓) ->
+    Γ.length ∉ fv e ->
+    typing Γ (.lam₂ e) (.rep (.arrow τ𝕒 τ𝕓))
+  | app₁ : ∀ Γ f arg τ𝕒 τ𝕓,
+    typing Γ f (.arrow τ𝕒 τ𝕓) ->
+    typing Γ arg τ𝕒 ->
+    typing Γ (.app₁ f arg) τ𝕓
+  | app₂ : ∀ Γ f arg τ𝕒 τ𝕓,
+    typing Γ f (.rep (.arrow τ𝕒 τ𝕓)) ->
+    typing Γ arg (.rep τ𝕒) ->
+    typing Γ (.app₂ f arg) (.rep τ𝕓)
+  | plus₁ : ∀ Γ l r,
+    typing Γ l .nat ->
+    typing Γ r .nat ->
+    typing Γ (.plus₁ l r) .nat
+  | plus₂ : ∀ Γ l r,
+    typing Γ l (.rep .nat) ->
+    typing Γ r (.rep .nat) ->
+    typing Γ (.plus₂ l r) (.rep .nat)
+  | lit₁ : ∀ Γ n,
+    typing Γ (.lit₁ n) .nat
+  | lit₂ : ∀ Γ n,
+    typing Γ (.lit₂ n) (.rep .nat)
+  | code : ∀ Γ e τ,
+    typing Γ e τ ->
+    typing Γ (.code e) (.rep τ)
+  | reflect : ∀ Γ e τ,
+    typing Γ e τ ->
+    typing Γ (.reflect e) (.rep τ)
+  | lam𝕔 : ∀ Γ e τ𝕒 τ𝕓,
+    typing (τ𝕒 :: Γ) (open₀ Γ.length e) (.rep τ𝕓) ->
+    Γ.length ∉ fv e ->
+    typing Γ (.lam𝕔 e) (.rep (.arrow τ𝕒 τ𝕓))
+  | lets : ∀ Γ b e τ𝕒 τ𝕓,
+    typing Γ b τ𝕒 ->
+    typing (τ𝕒 :: Γ) (open₀ Γ.length e) τ𝕓 ->
+    Γ.length ∉ fv e ->
+    typing Γ (.lets b e) τ𝕓
+  | let𝕔 : ∀ Γ b e τ𝕒 τ𝕓,
+    typing Γ b τ𝕒 ->
+    typing (τ𝕒 :: Γ) (open₀ Γ.length e) (.rep τ𝕓) ->
+    Γ.length ∉ fv e ->
+    typing Γ (.let𝕔 b e) (.rep τ𝕓)
 
 example : typing [] (.lam₁ (.bvar 0)) (.arrow .nat .nat) := by apply typing.lam₁; simp; apply typing.fvar; simp; simp
 
